src/impl/TLS13.Impl.Server.Network.fsti
@@ -192,4 +192,5 @@ fn process_network_bytes
                    network_out_bytes
                    app_out_bytes /\
                 (buffer_resp.ST.response.ST.status == ST.NeedMoreInput ==>
-                  W.parse_record_wire (Ghost.reveal 'raw_bytes) == None))
+                  W.parse_record_wire (Ghost.reveal 'raw_bytes) == None /\
+                  Seq.equal network_out_bytes (Ghost.reveal 'old_network_out)))
